Base Kappa on structural arrow instance
- This is faster(?) than using a typeclass arrow during generation as
typeclass resolution doesn't need to occur everywhere
- The constructive arrow instance can be cast to any typeclass Cava
instance via `toCava`
- Encoding of structural equivalence as an inductive type should allow
efficient structural equivalences

cava/arrow-examples/ArrowExamplesSV.hs
@@ -18,6 +18,7 @@ module Main where
 
 import Cava2SystemVerilog
 import ArrowExamples
+import Mux2_1
 
 main :: IO ()
 main = do writeSystemVerilog nandArrow
@@ -26,3 +27,4 @@ main = do writeSystemVerilog nandArrow
           writeTestBench arrow_xor_tb
           writeSystemVerilog feedbackNandArrow
           writeTestBench feedbackNandArrow_tb
+          writeSystemVerilog mux2_1_netlist
