cava/cava/Cava/Arrow.v
@@ -1,6 +1,6 @@
 Require Export Cava.Arrow.Arrow.
+Require Export Cava.Arrow.Instances.Constructive.
 Require Export Cava.Arrow.Instances.Combinational.
 Require Export Cava.Arrow.Instances.Netlist.
-(* Require Export Cava.Arrow.Instances.Stream. *)
 
 Require Export Cava.Arrow.Kappa.Syntax.
